theories/MetaTheory/Confluence.v
@@ -1,0 +1,9 @@
+From Metaprog Require Import Prelude Data.Term Data.Context MetaTheory.Reduction.
+
+(** This module proves the confluence lemma for the reduction relation [red]. *)
+
+Lemma red_confluence {s} (t u1 u2 : term s) :
+  red t u1 ->
+  red t u2 ->
+  exists v, red u1 v /\ red u2 v.
+Proof. Admitted.
