theories/MetaTheory/Reduction.v
@@ -1,0 +1,232 @@
+From Metaprog Require Import Prelude Data.Term Data.Context.
+
+(** This module defines:
+    - The one-step strong reduction relation [red1] on [term].
+    - The reduction relation [red] on [term] and its basic properties. *)
+
+(***********************************************************************)
+(** * One-step reduction relation [red1]. *)
+(***********************************************************************)
+
+Unset Elimination Schemes.
+
+(** Strong one-step reduction relation. This relation is _not_ deterministic. *)
+Inductive red1 {s} : term s -> term s -> Prop :=
+
+(** Beta-reduction rule. *)
+| red1_beta x ty body arg args :
+    red1 (TApp (TLam x ty body) (arg :: args)) (TApp (body[x := arg]) args)
+
+(** Congrence rules for [TLam]. *)
+| red1_lam_l x ty ty' body :
+    red1 ty ty' -> red1 (TLam x ty body) (TLam x ty' body)
+| red1_lam_r x ty body body' :
+    red1 body body' -> red1 (TLam x ty body) (TLam x ty body')
+
+(** Congruence rules for [TProd]. *)
+| red1_prod_l x a a' b :
+    red1 a a' -> red1 (TProd x a b) (TProd x a' b)
+| red1_prod_r x a b b' :
+    red1 b b' -> red1 (TProd x a b) (TProd x a b')
+
+(** Congruence rules for [TApp]. *)
+| red1_app_l f f' args :
+    red1 f f' -> red1 (TApp f args) (TApp f' args)
+| red1_app_r f args args' :
+    OnOne2 red1 args args' -> red1 (TApp f args) (TApp f args').
+
+Set Elimination Schemes.
+
+Derive Signature for red1.
+
+(** Induction principle for [red1]. We can't use Rocq's default induction principle
+    because [red1] is nested over [OnOne2]. *)
+Lemma red1_ind (P : forall s, term s -> term s -> Prop) :
+  (forall s x ty body arg args,
+    P s (TApp (TLam x ty body) (arg :: args)) (TApp (body[x := arg]) args)) ->
+  (forall s x ty ty' body,
+    red1 ty ty' ->
+    P s ty ty' ->
+    P s (TLam x ty body) (TLam x ty' body)) ->
+  (forall s x ty body body',
+    red1 body body' ->
+    P (s ▷ x) body body' ->
+    P s (TLam x ty body) (TLam x ty body')) ->
+  (forall s x a a' b,
+    red1 a a' ->
+    P s a a' ->
+    P s (TProd x a b) (TProd x a' b)) ->
+  (forall s x a b b',
+    red1 b b' ->
+    P (s ▷ x) b b' ->
+    P s (TProd x a b) (TProd x a b')) ->
+  (forall s f f' args,
+    red1 f f' ->
+    P s f f' ->
+    P s (TApp f args) (TApp f' args)) ->
+  (forall s f args args',
+    OnOne2 (fun arg arg' => red1 arg arg' /\ P s arg arg') args args' ->
+    P s (TApp f args) (TApp f args')) ->
+  forall s t t', red1 t t' -> P s t t'.
+Proof.
+intros Hbeta Hlam_l Hlam_r Hprod_l Hprod_r Happ_l Happ_r. fix IH 4.
+intros s t t' Hred. destruct Hred.
+- apply Hbeta.
+- apply Hlam_l ; auto.
+- apply Hlam_r ; auto.
+- apply Hprod_l ; auto.
+- apply Hprod_r ; auto.
+- apply Happ_l ; auto.
+- apply Happ_r. revert args args' H. fix IHargs 3. intros args args' H. destruct H.
+  + constructor. split ; auto.
+  + constructor. now apply IHargs.
+Qed.
+
+(***********************************************************************)
+(** * Reduction relation [red]. *)
+(***********************************************************************)
+
+(** Strong reduction relation, defined as the reflexive-transitive closure of [red1]. *)
+Inductive red {s} : term s -> term s -> Prop :=
+| red_of_red1 t1 t2 : red1 t1 t2 -> red t1 t2
+| red_refl t : red t t
+| red_trans t1 t2 t3 : red t1 t2 -> red t2 t3 -> red t1 t3.
+
+Derive Signature for red.
+
+#[export] Instance red_Reflexive s : Reflexive (@red s).
+Proof. intros t. apply red_refl. Qed.
+
+#[export] Instance red_Transitive s : Transitive (@red s).
+Proof. intros t1 t2 t3. apply red_trans. Qed.
+
+(***********************************************************************)
+(** * Congruence lemmas. *)
+(***********************************************************************)
+
+Section CongruenceLemmas.
+  Context {s : scope}.
+
+  Lemma red_beta x (ty : term s) body arg args :
+    red (TApp (TLam x ty body) (arg :: args)) (TApp (body[x := arg]) args).
+  Proof. apply red_of_red1. constructor. Qed.
+
+  Lemma red_lam_congr x (ty ty' : term s) body body' :
+    red ty ty' ->
+    red body body' ->
+    red (TLam x ty body) (TLam x ty' body').
+  Proof.
+  intros Hty Hbody. transitivity (TLam x ty body').
+  - clear Hty. induction Hbody.
+    + apply red_of_red1. now constructor.
+    + reflexivity.
+    + etransitivity ; eauto.
+  - clear Hbody. induction Hty.
+    + apply red_of_red1. now constructor.
+    + reflexivity.
+    + etransitivity ; eauto.
+  Qed.
+
+  Lemma red_prod_congr x (a a' : term s) b b' :
+    red a a' ->
+    red b b' ->
+    red (TProd x a b) (TProd x a' b').
+  Proof.
+  intros Ha Hb. transitivity (TProd x a b').
+  - clear Ha. induction Hb.
+    + apply red_of_red1. now constructor.
+    + reflexivity.
+    + etransitivity ; eauto.
+  - clear Hb. induction Ha.
+    + apply red_of_red1. now constructor.
+    + reflexivity.
+    + etransitivity ; eauto.
+  Qed.
+
+  Lemma red_app_congr (f f' : term s) args args' :
+    red f f' ->
+    All2 red args args' ->
+    red (TApp f args) (TApp f' args').
+  Proof.
+  intros Hf Hargs. transitivity (TApp f' args).
+  - clear Hargs. induction Hf.
+    + apply red_of_red1. now constructor.
+    + reflexivity.
+    + etransitivity ; eauto.
+  - clear f Hf.
+
+  Admitted.
+
+End CongruenceLemmas.
+
+(***********************************************************************)
+(** * Inversion lemmas. *)
+(***********************************************************************)
+
+Section InversionLemmas.
+  Context {s : scope}.
+
+  Lemma red_type_inv (t : term s) :
+    red TType t -> t = TType.
+  Proof.
+  intros H. depind H.
+  - depelim H.
+  - reflexivity.
+  - subst. specialize (IHred2 t3 eq_refl). now subst.
+  Qed.
+
+  Lemma red_var_inv (i : index s) (t : term s) :
+    red (TVar i) t -> t = TVar i.
+  Proof.
+  intros H. depind H.
+  - depelim H.
+  - reflexivity.
+  - subst. specialize (IHred2 i t3 eq_refl). now subst.
+  Qed.
+
+  Lemma red_lam_inv x (ty : term s) body t :
+    red (TLam x ty body) t ->
+    exists ty' body',
+      t = TLam x ty' body' /\
+      red ty ty' /\
+      red body body'.
+  Proof.
+  intros Hred. depind Hred.
+  - depelim H.
+    + exists ty', body. split3 ; [reflexivity | now apply red_of_red1 | reflexivity].
+    + exists ty, body'. split3 ; [reflexivity | reflexivity | now apply red_of_red1].
+  - exists ty, body. now split3.
+  - destruct IHHred1 as (ty' & body' & -> & Hty1 & Hbody1).
+    specialize (IHHred2 x ty' body' t3 eq_refl).
+    destruct IHHred2 as (ty'' & body'' & -> & Hty2 & Hbody2).
+    exists ty'', body''. split3 ; [reflexivity | etransitivity ; eauto ..].
+  Qed.
+
+  Lemma red_prod_inv x (a : term s) b t :
+    red (TProd x a b) t ->
+    exists a' b',
+      t = TProd x a' b' /\
+      red a a' /\
+      red b b'.
+  Proof.
+  intros Hred. depind Hred.
+  - depelim H.
+    + exists a', b. split3 ; [reflexivity | now apply red_of_red1 | reflexivity].
+    + exists a, b'. split3 ; [reflexivity | reflexivity | now apply red_of_red1].
+  - exists a, b. now split3.
+  - destruct IHHred1 as (a' & b' & -> & Ha1 & Hb1).
+    specialize (IHHred2 x a' b' t3 eq_refl).
+    destruct IHHred2 as (a'' & b'' & -> & Ha2 & Hb2).
+    exists a'', b''. split3 ; [reflexivity | etransitivity ; eauto ..].
+  Qed.
+
+  Lemma red_evar_inv ev (t : term s) :
+    red (TEvar ev) t -> t = TEvar ev.
+  Proof.
+  intros H. depind H.
+  - depelim H.
+  - reflexivity.
+  - subst. specialize (IHred2 ev t3 eq_refl). now subst.
+  Qed.
+
+End InversionLemmas.
